Leanr/Implementation/Optimizer.lean
@@ -13,6 +13,7 @@ import Leanr.Implementation.OptimizerPasses.TautoBus
 import Leanr.Implementation.OptimizerPasses.MonicScale
 import Leanr.Implementation.OptimizerPasses.MemoryUnify
 import Leanr.Implementation.OptimizerPasses.BusUnify
+import Leanr.Implementation.OptimizerPasses.BusPairCancel
 import Leanr.Implementation.OptimizerPasses.DisconnectedComponent
 import Leanr.Implementation.OptimizerPasses.Reencode
 
@@ -60,6 +61,7 @@ def cleanupCycle : VerifiedPassW p :=
     |>.andThen zeroMultBusDropPass.withFacts.guardDegree
     |>.andThen tautoBusDropPass.withFacts.guardDegree
     |>.andThen busUnifyPass.guardDegree
+    |>.andThen (VerifiedPassW.guardDegree (iterateToFixpoint busPairCancelPass))
     |>.andThen disconnectedComponentPass.withFacts.guardDegree
     |>.andThen reencodePass.withFacts.guardDegree
 
